some changes I don't recall + rt analysis

theories/L/Complexity/Cook/FlatPR_to_BinaryPR.v
@@ -145,3 +145,308 @@ Proof.
     eapply PR_wf_dec_correct, isFlatPROf_wf_equivalent; easy.
 Qed.
 
+
+(** *extraction *)
+From Undecidability.L.Tactics Require Import LTactics GenEncode.
+From Undecidability.L.Datatypes Require Import  LProd LOptions LBool LLNat LLists.
+From Undecidability.L.Complexity Require Import PolyBounds. 
+
+(*repEl *)
+Section fixX. 
+  Context {X : Type}.
+  Context `{H: registered X}. 
+
+  Definition c__repEl2 := 5.
+  Definition c__repEl := c__repEl2 + 7.
+  Definition repEl_time (n: nat) := (n +1) * c__repEl. 
+  Global Instance term_repEl : computableTime' (@repEl X) (fun n _ => (c__repEl2, fun e _ => (repEl_time n, tt))). 
+  Proof. 
+    extract. solverec. all: unfold repEl_time, c__repEl, c__repEl2; solverec.
+  Defined. 
+
+  Lemma repEl_time_mono : monotonic repEl_time. 
+  Proof. 
+    unfold repEl_time; smpl_inO. 
+  Qed. 
+
+  Definition poly__repEl n := (n+1) * c__repEl.
+  Lemma repEl_time_bound n : repEl_time n <= poly__repEl (size (enc n)). 
+  Proof. 
+    unfold repEl_time, poly__repEl. replace_le n with (size (enc n)) by (apply size_nat_enc_r) at 1. lia. 
+  Qed. 
+  Lemma repEl_poly : monotonic poly__repEl /\ inOPoly poly__repEl. 
+  Proof. 
+    unfold poly__repEl; split; smpl_inO. 
+  Qed. 
+End fixX. 
+
+(*hNat *)
+Definition c__hNat := 2 * (c__leb2 + 2 * c__repEl2 + 82).
+Definition hNat_time sig n := (leb_time (S n) sig + repEl_time sig + sig + 1) * c__hNat. 
+Instance term_hNat : computableTime' hNat (fun sig _ => (1, fun n _ => (hNat_time sig n, tt))). 
+Proof. 
+  specialize (repEl_time_mono) as H1. unfold monotonic in H1. 
+  extract. solverec. 
+  - setoid_rewrite Nat.le_min_r at 2. rewrite Nat.mul_1_r. rewrite repEl_length. 
+    apply leb_iff in H. rewrite H1 with (x' := x) by lia. setoid_rewrite H1 with (x' := x) at 2. 2: lia. 
+    rewrite Nat.le_min_l. 
+    unfold hNat_time, c__hNat. cbn[Nat.add]. nia. 
+  - cbn[Nat.add]. unfold hNat_time, c__hNat. apply Nat.leb_gt in H. 
+    unfold repEl_time. nia. 
+Qed. 
+
+Definition c__hNatBound := (c__leb + 1) * (c__hNat + 1).
+Definition poly__hNat n := (poly__repEl n + n + 1) * c__hNatBound.
+Lemma hNat_time_bound sig n: hNat_time sig n <= poly__hNat (size (enc sig)). 
+Proof. 
+  unfold hNat_time. rewrite leb_time_bound_r. 
+  unfold poly__hNat, c__hNatBound. rewrite repEl_time_bound. rewrite size_nat_enc_r with (n := sig) at 3.
+  leq_crossout. 
+Qed. 
+Lemma hNat_poly : monotonic poly__hNat /\ inOPoly poly__hNat. 
+Proof.
+  unfold poly__hNat; split; smpl_inO; apply repEl_poly. 
+Qed. 
+
+(*concat *)
+Section concat_fixX. 
+  Context {X : Type}.
+  Context `{registered X}.
+  
+  Definition c__concat := 19.
+  Definition concat_time (l : list (list X)) := fold_right (fun l acc => c__concat * (|l|) + acc + c__concat) c__concat l.
+  Global Instance term_concat : computableTime' (@concat X) (fun l _ => (concat_time l, tt)). 
+  Proof. 
+    extract. unfold concat_time, c__concat. solverec. 
+  Qed. 
+  
+  Definition poly__concat n := (n + 1) * c__concat.
+  Lemma concat_time_bound l : concat_time l <= poly__concat (size (enc l)). 
+  Proof. 
+    unfold concat_time. induction l; cbn -[Nat.add Nat.mul].
+    - unfold poly__concat. nia. 
+    - rewrite IHl. unfold poly__concat. rewrite list_size_cons. rewrite list_size_length. nia.
+  Qed. 
+  Lemma concat_poly : monotonic poly__concat /\ inOPoly poly__concat. 
+  Proof. 
+    split; unfold poly__concat; smpl_inO. 
+  Qed. 
+End concat_fixX. 
+
+(*hflat *)
+Definition c__hflat := c__Sigma + 3. 
+Definition hflat_time (fpr : FlatPR) (l : list nat) := map_time (fun m => hNat_time (Sigma fpr) m) l + concat_time (map (hNat (Sigma fpr)) l) + c__hflat.
+Instance term_hflat : computableTime' hflat (fun fpr _ => (1, fun l _ => (hflat_time fpr l, tt))).  
+Proof. 
+  unfold hflat. unfold canonicalHom. extract. solverec. 
+  unfold hflat_time, c__hflat. solverec. 
+Qed. 
+
+Definition c__hNatSize := 9.
+Lemma hNat_size_bound sig n: size (enc (hNat sig n)) <= (sig + 1) * c__hNatSize. 
+Proof. 
+  specialize (list_size_of_el (l := (hNat sig n)) (k := 4)) as H1.  
+  rewrite H1. 2: { intros. apply size_bool. }
+  rewrite hNat_length. unfold c__hNatSize. lia. 
+Qed. 
+
+Lemma map_hNat_size_bound sig l : size (enc (map (hNat sig) l)) <= (|l|) * (sig + 1) * c__hNatSize + 5 * (|l|) + 4. 
+Proof. 
+  erewrite list_size_of_el. 
+  2: { intros a H%in_map_iff. destruct H as (n & <- & H). apply hNat_size_bound. }
+  rewrite map_length. lia. 
+Qed. 
+
+Definition c__hflatBound := (c__hNatSize + 5) * (c__concat + 1) + c__hflat + 1 + (c__map + 1). 
+Definition poly__hflat n := ((n + 1) * (poly__hNat n + 1) + ((n+1) * (n+1) + n + 1) + 1) * c__hflatBound.
+Lemma hflat_time_bound fpr l : hflat_time fpr l <= poly__hflat (size (enc fpr) + size (enc l)).
+Proof. 
+  unfold hflat_time. rewrite map_time_bound_env. 
+  2: { 
+    split; [ intros | ]. 
+    - rewrite hNat_time_bound. poly_mono hNat_poly. 2: apply Nat.le_add_r with (m := size (enc ele)). reflexivity. 
+    - apply hNat_poly. 
+    } 
+  poly_mono hNat_poly. 
+  2: (replace_le (size (enc (Sigma fpr))) with (size (enc fpr)) by (rewrite FlatPR_enc_size; lia)); reflexivity.
+
+  rewrite concat_time_bound. poly_mono concat_poly. 
+  2: { 
+    rewrite map_hNat_size_bound. rewrite list_size_length. 
+    replace_le (Sigma fpr) with (size (enc fpr)) by (rewrite size_nat_enc_r with (n := Sigma fpr); rewrite FlatPR_enc_size; lia). 
+    reflexivity. 
+  } 
+  unfold poly__concat. 
+  rewrite list_size_length.
+  unfold poly__hflat, c__hflatBound. unfold c__hNatSize, c__concat, c__hflat, c__map. nia. 
+Qed. 
+Lemma hflat_poly : monotonic poly__hflat /\ inOPoly poly__hflat.    
+Proof. 
+  split; unfold poly__hflat; smpl_inO; apply hNat_poly. 
+Qed. 
+
+Lemma hflat_length fpr l : |hflat fpr l| = (Sigma fpr) * |l|. 
+Proof. 
+  induction l; cbn; [lia | ]. 
+  rewrite app_length, hNat_length. unfold hflat, canonicalHom in IHl. rewrite IHl. 
+  nia.
+Qed. 
+
+Lemma hflat_size_bound fpr l : size (enc (hflat fpr l)) <= 9 * (|l|) * (Sigma fpr) + 4. 
+Proof. 
+  rewrite list_size_of_el by (intros; apply size_bool).
+  rewrite hflat_length. nia.
+Qed. 
+
+(*hwindow *)
+Definition c__hwindow := 9. 
+Definition hwindow_time (fpr : FlatPR) (win : PRWin nat) := hflat_time fpr (prem win) + hflat_time fpr (conc win) + c__hwindow. 
+Instance term_hwindow : computableTime' hwindow (fun fpr _ => (1, fun win _ => (hwindow_time fpr win, tt))). 
+Proof. 
+  extract. solverec. unfold hwindow_time, c__hwindow. solverec. 
+Defined. 
+
+Definition poly__hwindow n := poly__hflat n + poly__hflat n + c__hwindow. 
+Lemma hwindow_time_bound fpr win : hwindow_time fpr win <= poly__hwindow (size (enc fpr) + size (enc win)).
+Proof. 
+  unfold hwindow_time. rewrite !hflat_time_bound. 
+  unfold poly__hwindow. 
+  poly_mono hflat_poly. 2: { replace_le (size (enc (prem win))) with (size (enc win)) by (rewrite PRWin_enc_size; lia). reflexivity. }
+  poly_mono hflat_poly at 2. 2: { replace_le (size (enc (conc win))) with (size (enc win)) by (rewrite PRWin_enc_size; lia). reflexivity. }
+  lia. 
+Qed. 
+Lemma hwindow_poly : monotonic poly__hwindow /\ inOPoly poly__hwindow. 
+Proof. 
+  unfold poly__hwindow; split; smpl_inO; apply hflat_poly. 
+Qed. 
+
+(*Lemma hwindow_size_bound fpr l : size (enc (hflat*)
+
+(*hwindows *)
+Definition c__hwindows := c__windows + 3. 
+Definition hwindows_time (fpr : FlatPR) := map_time (fun w => hwindow_time fpr w) (windows fpr) + c__hwindows.
+Instance term_hwindows : computableTime' hwindows (fun fpr _ => (hwindows_time fpr, tt)). 
+Proof. 
+  extract. solverec. unfold hwindows_time, c__hwindows. solverec. 
+Defined. 
+
+Definition c__hwindowsBound := (c__hwindows + 1) * (c__map + 1).
+Definition poly__hwindows n :=  ((n + 1) * (poly__hwindow (n+ n) + 1) + 1) * c__hwindowsBound.
+Lemma hwindows_time_bound fpr : hwindows_time fpr <= poly__hwindows (size (enc fpr)). 
+Proof. 
+  unfold hwindows_time. 
+  rewrite map_time_bound_env. 2: split; [ intros; apply hwindow_time_bound | apply hwindow_poly]. 
+  rewrite list_size_length. 
+  replace_le (size (enc (windows fpr))) with (size (enc fpr)) by (rewrite FlatPR_enc_size; lia) at 1. 
+  poly_mono hwindow_poly. 
+  2: { replace_le (size (enc (windows fpr))) with (size (enc fpr)) by (rewrite FlatPR_enc_size; lia) at 1. reflexivity. }
+  unfold poly__hwindows, c__hwindowsBound. nia.
+Qed. 
+Lemma hwindows_poly : monotonic poly__hwindows /\ inOPoly poly__hwindows. 
+Proof. 
+  unfold poly__hwindows; split; smpl_inO. 
+  - apply hwindow_poly. 
+  - eapply inOPoly_comp; [apply hwindow_poly | apply hwindow_poly | smpl_inO].
+Qed. 
+
+(*hfinal *)
+Definition c__hfinal := c__final + 3. 
+Definition hfinal_time (fpr : FlatPR) := map_time (fun l => hflat_time fpr l) (final fpr) + c__hfinal. 
+Instance term_hfinal : computableTime' hfinal (fun fpr _ => (hfinal_time fpr, tt)). 
+Proof. 
+  extract. solverec. unfold hfinal_time, c__hfinal; solverec. 
+Defined.
+
+Definition c__hfinalBound := (c__hfinal + 1) * (c__map + 1).
+Definition poly__hfinal n :=  ((n + 1) * (poly__hflat (n+ n) + 1) + 1) * c__hfinalBound.
+Lemma hfinal_time_bound fpr : hfinal_time fpr <= poly__hfinal (size (enc fpr)). 
+Proof. 
+  unfold hfinal_time. 
+  rewrite map_time_bound_env. 2: split; [ intros; apply hflat_time_bound | apply hflat_poly]. 
+  rewrite list_size_length. 
+  replace_le (size (enc (final fpr))) with (size (enc fpr)) by (rewrite FlatPR_enc_size; lia) at 1. 
+  poly_mono hflat_poly. 
+  2: { replace_le (size (enc (final fpr))) with (size (enc fpr)) by (rewrite FlatPR_enc_size; lia) at 1. reflexivity. }
+  unfold poly__hfinal, c__hfinalBound. nia.
+Qed. 
+Lemma hfinal_poly : monotonic poly__hfinal /\ inOPoly poly__hfinal. 
+Proof. 
+  unfold poly__hfinal; split; smpl_inO. 
+  - apply hflat_poly. 
+  - eapply inOPoly_comp; [apply hflat_poly | apply hflat_poly | smpl_inO].
+Qed. 
+
+(*hBinaryPR *)
+Definition c__hBinaryPR := 2 * c__Sigma + c__offset + c__width + c__init + c__windows + c__steps + 28.
+Definition c__hBinaryPR2 := 38.
+Definition hBinaryPR_time (fpr : FlatPR) := c__hBinaryPR2 * (Sigma fpr * offset fpr + Sigma fpr * width fpr + Sigma fpr + hflat_time fpr (init fpr) + hwindows_time fpr + hfinal_time fpr) + c__hBinaryPR.
+Instance term_hBinaryPR : computableTime' hBinaryPR (fun fpr _ => (hBinaryPR_time fpr, tt)).
+Proof. 
+  unfold hBinaryPR. unfold hoffset, hwidth, hsteps, hinit.  
+  extract. solverec. 
+  unfold hBinaryPR_time, c__hBinaryPR, c__hBinaryPR2. solverec. 
+Defined. 
+
+Definition poly__hBinaryPR n := c__hBinaryPR2 * (2 * n * n + n + poly__hflat (n +n) + poly__hwindows n + poly__hfinal n) + c__hBinaryPR. 
+Lemma hBinaryPR_time_bound fpr : hBinaryPR_time fpr <= poly__hBinaryPR (size (enc fpr)). 
+Proof. 
+  unfold hBinaryPR_time. 
+  replace_le (Sigma fpr) with (size (enc fpr)) by (rewrite size_nat_enc_r, FlatPR_enc_size; lia). 
+  replace_le (offset fpr) with (size (enc fpr)) by (rewrite size_nat_enc_r, FlatPR_enc_size; lia).
+  replace_le (width fpr) with (size (enc fpr)) by (rewrite size_nat_enc_r, FlatPR_enc_size; lia).
+  rewrite hflat_time_bound. 
+  poly_mono hflat_poly. 
+  2: { (replace_le (size (enc (init fpr))) with (size (enc fpr)) by (rewrite FlatPR_enc_size; lia)); reflexivity. }
+  rewrite hfinal_time_bound. rewrite hwindows_time_bound. 
+  unfold poly__hBinaryPR. nia. 
+Qed. 
+Lemma hBinaryPR_poly : monotonic poly__hBinaryPR /\ inOPoly poly__hBinaryPR. 
+Proof. 
+  split; unfold poly__hBinaryPR; smpl_inO. all: try solve [apply hflat_poly  | apply hwindows_poly | apply hfinal_poly ].
+  eapply inOPoly_comp; [apply hflat_poly | apply hflat_poly | smpl_inO].
+Qed. 
+
+(*reduction *)
+Definition c__reduction := 9. 
+Definition reduction_time (fpr : FlatPR) := FlatPR_wf_dec_time fpr + isValidFlattening_dec_time fpr + hBinaryPR_time fpr + c__reduction.
+Local Instance term_reduction : computableTime' reduction (fun fpr _ => (reduction_time fpr, tt)).
+Proof. 
+  extract. solverec. all: unfold reduction_time, c__reduction; solverec. 
+Defined.  
+
+Definition poly__reduction n := poly__FlatPRWfDec n + poly__isValidFlatteningDec n + poly__hBinaryPR n + c__reduction. 
+Lemma reduction_time_bound fpr : reduction_time fpr <= poly__reduction (size (enc fpr)). 
+Proof. 
+  unfold reduction_time, poly__reduction. 
+  rewrite FlatPR_wf_dec_time_bound, isValidFlattening_dec_time_bound, hBinaryPR_time_bound. lia. 
+Qed. 
+Lemma reduction_poly : monotonic poly__reduction /\ inOPoly poly__reduction. 
+Proof. 
+  split; unfold poly__reduction; smpl_inO. 
+  all: try solve [ apply FlatPR_wf_dec_poly | apply isValidFlatteningDec_poly | apply hBinaryPR_poly]. 
+Qed. 
+
+(*size bound *)
+Lemma reduction_size_bound fpr : exists f, size (enc (reduction fpr)) <= f (size (enc fpr)) /\ inOPoly f /\ monotonic f.
+Proof. 
+  evar (f : nat -> nat). exists f. split; [ | split]. 
+  + unfold reduction. destruct andb. 
+    - unfold hBinaryPR. rewrite BinaryPR_enc_size; cbn. 
+      rewrite !size_nat_enc. 
+
+Lemma FlatPR_to_BinaryPR_poly : reducesPolyMO (unrestrictedP FlatPRLang) (unrestrictedP BinaryPRLang).
+Proof. 
+  exists reduction.
+  - exists poly__reduction. 
+    + constructor. 
+      extract.  solverec. 
+      all: specialize (reduction_time_bound x) as H1; unfold reduction_time, c__reduction in H1; nia.
+    + apply reduction_poly.
+    + apply reduction_poly. 
+    + evar (f : nat -> nat). exists f. split; [ | split]. 
+      * intros fpr. unfold reduction. 
+
+
+  
+
+
