theories/L/Complexity/PolyBounds.v
@@ -73,7 +73,6 @@ Proof.
     solverec. 
 Qed. 
 
-
 Tactic Notation "replace_le" constr(s) "with" constr(r) "by" tactic(tac) :=
   let H := fresh in assert (s <= r) as H by tac; rewrite !H; clear H. 
 Tactic Notation "replace_le" constr(s) "with" constr(r) "by" tactic(tac) "at" integer(occ) := 
@@ -143,38 +142,22 @@ Section fixX.
 
    *)
 
-  (* Lemma dupfreeb_time_bound_env (eqbT : Y -> X -> X -> nat) (f : nat -> nat): *)
-  (*   (forall (a b : X) (y : Y), eqbT y a b <= f (size (enc a) + size (enc b) + size(enc y))) /\ monotonic f *)
-  (*    -> forall (l : list X) (y : Y), dupfreeb_time (eqbT y) l <= (|l| + 1) * (f (size (enc l) + size (enc y)) + c__dupfreeb).  *)
-  (* Proof.  *)
-  (*   intros [H1 H2]. intros. induction l.  *)
-  (*   - cbn. lia.  *)
-  (*   - cbn. rewrite IHl. rewrite list_in_decb_time_bound_env by easy.   *)
-  (*     unfold monotonic in H2. erewrite H2. *)
-  (*     2: (replace_le (size (enc l) + size (enc a)) with (size (enc (a::l))) by (rewrite list_size_cons; lia)); reflexivity. *)
-  (*     setoid_rewrite H2 at 2.  *)
-  (*     2: (replace_le (size(enc l)) with (size (enc (a::l))) by (rewrite list_size_cons; lia)); reflexivity. *)
-  (*     nia.  *)
-
-  (* Lemma dupfreeb_time_bound_env (eqbT : Y -> X -> X -> nat): *)
-  (*   (* eqbT is polynomial in encoding of a and b and the environment y *) *)
-  (*   (exists (f : nat -> nat), (forall (a b : X) (y : Y), eqbT y a b <= f (size(enc a) + size(enc b) + size(enc y))) /\ inOPoly f /\ monotonic f) *)
-  (*   -> exists (f : nat -> nat), (forall (l : list X) (y : Y), dupfreeb_time (eqbT y) l <= f (size(enc l) + size(enc y))) /\ inOPoly f /\ monotonic f. *)
-  (* Proof. *)
-  (*   intros H1. *)
-  (*   specialize (list_in_decb_time_bound_env H1) as (f_indec & F1 & F2 & F3). *)
-  (*   destruct H1 as (f' & H1 & H2). *)
-  (*   evar (f : nat -> nat). exists f. split; try split. *)
-  (*   1:{ intros l y. unfold dupfreeb_time. *)
-  (*     instantiate (f := fun n => n * f_indec (n) + c__dupfreeb *n + c__dupfreeb). subst f. *)
-  (*     induction l. *)
-  (*     + lia. *)
-  (*     + rewrite IHl. rewrite F1. clear IHl. solverec. rewrite list_size_cons. *)
-  (*       unfold monotonic in F3. rewrite F3 with (x' := size(enc a) + size(enc l) +5 + size(enc y)). 2:lia. *)
-  (*       rewrite F3 with (x := size(enc l) + size(enc y)) (x' := size (enc a) + size(enc l) + 5 + size(enc y)). solverec. lia. *)
-  (*     } *)
-  (*   all: subst f; smpl_inO. *)
-  (* Qed. *)
+  Definition c__dupfreeBound := c__dupfreeb + c__list_in_decb. 
+  Lemma dupfreeb_time_bound_env (eqbT : Y -> X -> X -> nat) (f : nat -> nat): 
+    (forall (a b : X) (y : Y), eqbT y a b <= f (size (enc a) + size (enc b) + size(enc y))) /\ monotonic f 
+     -> forall (l : list X) (y : Y), dupfreeb_time (eqbT y) l <= (|l| + 1) * (|l| + 1) * (f (2* size (enc l) + size (enc y)) + c__dupfreeBound). 
+  Proof.  
+    intros [H1 H2]. intros. induction l.  
+    - unfold c__dupfreeBound. cbn -[Nat.add]. lia.  
+    - cbn -[c__dupfreeBound c__list_in_decb]. rewrite IHl. rewrite list_in_decb_time_bound_env by easy.   
+      rewrite !Nat.add_0_r. 
+      unfold monotonic in H2. erewrite H2. 
+      2: (replace_le (size (enc l) + size (enc a)) with (size (enc (a::l)) + size(enc(a::l))) by (rewrite list_size_cons; lia)); reflexivity. 
+      setoid_rewrite H2 at 2.  
+      2: (replace_le (size(enc l)) with (size (enc (a::l))) by (rewrite list_size_cons; lia)); reflexivity. 
+      unfold c__dupfreeBound. cbn [Nat.mul]. rewrite !Nat.add_0_r. 
+      nia. 
+  Qed. 
 
   Lemma forallb_time_bound_env (predT : Y -> X -> nat) (f : nat -> nat):
     (forall (a : X) (y : Y), predT y a <= f (size(enc a) + size(enc y))) /\ monotonic f 
@@ -188,36 +171,24 @@ Section fixX.
       nia.
   Qed. 
 
-  (*Lemma forallb_time_bound_env (predT : Y -> X -> nat) :*)
-    (*(exists (f : nat -> nat), (forall (a : X) (y : Y), predT y a <= f (size(enc a) + size(enc y))) /\ inOPoly f /\ monotonic f)*)
-    (*-> exists (f : nat -> nat), (forall (l : list X) (y : Y), forallb_time (predT y) l <= f(size (enc l) + size(enc y)) ) /\ inOPoly f /\ monotonic f. *)
-  (*Proof. *)
-    (*intros (f' & H1 & H2 & H3). *)
-    (*evar (f : nat -> nat). exists f. split; try split.*)
-    (*1: {*)
-      (*intros l y. unfold forallb_time.*)
-      (*assert (forall (a : X) (l : list X) (y : Y), a el l -> predT y a <= f'(size (enc l) + size(enc y))).*)
-      (*{ clear l. intros a l y0 H4. rewrite H1. unfold monotonic in H3; rewrite H3.*)
-        (*2: { enough (size(enc a) + size(enc y0) <= size(enc l) + size (enc y0)) by apply H0. now rewrite list_el_size_bound. }*)
-        (*lia. }*)
-      (*instantiate (f := fun n => n * f' n + c__forallb * n + c__forallb). subst f.*)
-      (*induction l. *)
-      (*- cbn; lia. *)
-      (*- cbn -[ Nat.mul]. rewrite IHl. rewrite H0. 2: {assert (a el a :: l) by firstorder. apply H4. }*)
-      (*rewrite list_size_cons at 2. unfold monotonic in H3; rewrite H3 with (x:= size(enc l) + size(enc y)) (x' := size(enc(a::l)) + size(enc y)).  *)
-      (*rewrite list_size_cons at 4. solverec. *)
-      (*rewrite list_size_cons; lia. *)
-    (*}*)
-    (*all: unfold f; smpl_inO. *)
-  (*Qed. *)
-
-  Lemma nth_error_time_bound : exists (f : nat -> nat), (forall (l : list X) (n : nat), nth_error_time l <= f(size (enc l))) /\ inOPoly f /\ monotonic f. 
+  Lemma nth_error_time_bound : 
+    forall (l : list X) n, nth_error_time l n <= (min (size (enc l)) (size (enc n)) + 1) * c__ntherror.
   Proof.
-    evar (f : nat -> nat). exists f. split.
-    - intros. unfold nth_error_time. specialize (list_size_length l). 
-      instantiate (f := fun n => (c__ntherror) * (1 + n)). subst f. solverec. nia.
-    - subst f; split; smpl_inO. 
+    intros. unfold nth_error_time. rewrite size_nat_enc_r with (n := n) at 1. rewrite list_size_length. nia.
   Qed. 
+
+  Lemma map_time_bound_env (fT : Y -> X -> nat) (f__bound : nat -> nat): 
+    (forall (env : Y) (ele : X), fT env ele <= f__bound (size (enc env) + size (enc ele))) /\ monotonic f__bound
+    -> forall (env : Y) (l : list X), map_time (fT env) l <= (|l| + 1) * (f__bound (size (enc env) + size (enc l)) + 1) * (c__map + 1). 
+  Proof. 
+    intros [H1 H2] env l. induction l; cbn -[c__map]. 
+    - nia. 
+    - rewrite IHl. rewrite H1. unfold monotonic in H2. 
+      rewrite H2 at 1. 2: (replace_le (size (enc a)) with (size (enc (a::l))) by (rewrite list_size_cons; lia)); reflexivity. 
+      setoid_rewrite H2 at 2. 2: (replace_le (size (enc l)) with (size (enc (a::l))) by (rewrite list_size_cons; lia)); reflexivity. 
+      nia. 
+  Qed. 
+  
 End fixX.
 
 Section fixXY.
@@ -226,128 +197,43 @@ Section fixXY.
   Context {H0: registered Y}.
   Context {H1 : registered Z}.
 
-  (*the running time of foldr not only depends on the running time of the step function, *)
-  (*but also on the output size of the step function; in order to get a polynomial bound, *)
-  (*we require that this output size grows only by an additive constant in each step *)
-  Lemma fold_right_time_bound_env (step : Z -> Y -> X -> X) (stepT : Z -> (Y -> X -> nat)) :
-    (exists (f : nat -> nat), (forall (acc : X) (ele : Y) (env : Z), stepT env ele acc <= f(size(enc acc) + size(enc ele) + size(enc env))) /\ inOPoly f /\ monotonic f)
-    -> (exists (f_size :nat -> nat), (forall (acc : X) (ele : Y) (env : Z), size(enc (step env ele acc)) <= size(enc acc) + f_size (size(enc ele) + size(enc env))) /\ inOPoly f_size /\ monotonic f_size)
-    -> exists (f : nat -> nat), (forall (l : list Y) (acc : X) (env : Z), fold_right_time (step env) (stepT env) l acc <= f(size(enc l) + size(enc acc) + size(enc env))) /\ inOPoly f /\ monotonic f.
-  Proof.
-(*    intros (f__step & H2 & H3 & H4) (f_size & F1 & F2 & F3). *)
-    (*evar (f : nat -> nat). exists f. split.*)
-    (*- intros l init env.*)
-      (*[> we first show that the output size of foldr on every suffix is polynomial <]*)
-      (*assert (forall l' l'', l = l' ++ l'' -> size(enc (fold_right (step env) init l'')) <= size(enc init) + c__out' * size(enc l'') + (|l''|) * (c__out' * size(enc env) + c__out)).*)
-      (*{*)
-        (*intros l' l''; revert l'. induction l''.*)
-        (*+ cbn. intros; lia.*)
-        (*+ intros. cbn. rewrite F. rewrite IHl''. 2: { now rewrite app_comm_cons' in H5. }*)
-          (*rewrite list_size_cons. solverec. *)
-      (*}*)
+  Lemma fold_right_time_bound_env (step : Z -> Y -> X -> X) (stepT : Z -> Y -> X -> nat) (f__arg f__size : nat -> nat): 
+    (forall (acc : X) (ele : Y) (env : Z), stepT env ele acc <= f__arg (size (enc acc) + size (enc ele) + size (enc env))) /\ monotonic f__arg
+    -> (forall (acc : X) (ele : Y) (env : Z), size (enc (step env ele acc)) <= size (enc acc) + f__size (size (enc ele) + size (enc env))) /\ monotonic f__size
+    -> forall (l : list Y) (acc : X) (env : Z), fold_right_time (step env) (stepT env) l acc <= (|l| + 1) * f__arg (|l| * f__size (size(enc l) + size (enc env)) + size (enc acc) + size(enc l) + size (enc env)) + (|l| + 1) * c__fold_right. 
+  Proof. 
+    intros [G1 G2] [F1 F2] l init env. 
+    (*we first show that the output size of foldr on every suffix is bounded by |l| * fsize(size(enc l) + size(enc env)) + size(enc init) *)
+    assert (forall l' l'', l = l' ++ l'' -> size (enc (fold_right (step env) init l'')) <= |l''| * f__size(size (enc l'') + size (enc env)) + size (enc init)) as H3. 
+    { 
+      intros l' l''. revert l'. induction l''; intros.
+      - cbn. lia. 
+      - cbn. rewrite F1. rewrite IHl''. 2: { now rewrite app_comm_cons' in H2. } 
+        unfold monotonic in F2. setoid_rewrite F2 at 2. 
+        2: (replace_le (size(enc a)) with (size (enc (a::l''))) by (apply list_el_size_bound; eauto)); reflexivity. 
+        rewrite F2 at 1. 2: (replace_le (size (enc l'')) with (size (enc (a::l''))) by (rewrite list_size_cons; lia)); reflexivity. 
+        nia. 
+    } 
 
-      (*instantiate (f := fun n => 4 + n * f__step((S c__out) * (S c__out') * n * n + (S c__out') * n) + 15 * n). subst f.*)
-      (*unfold fold_right_time. *)
-      (*induction l.*)
-      (*+ solverec.*)
-      (*+ rewrite IHl, H2.*)
-        (** unfold monotonic in H4.*)
-          (*rewrite H4 with (x' := (S c__out) * (S c__out') * (size(enc(a::l)) + size(enc init) + size(enc env)) *  (size(enc(a::l)) + size(enc init) + size(enc env)) + (S c__out') * (size(enc(a::l)) + size(enc init) + size(enc env))). *)
-          (*2: {clear IHl. rewrite H5. rewrite list_size_length. rewrite list_size_cons.*)
-              (*2: {assert (a::l = [a] ++ l) as H6 by reflexivity; apply H6. }*)
-              (*cbn. rewrite Nat.mul_add_distr_l. nia. }*)
-
-          (*setoid_rewrite H4 with (x' := (S c__out) * (S c__out') * (size(enc(a::l)) + size(enc init) + size(enc env)) *  (size(enc(a::l)) + size(enc init) + size(enc env)) + (S c__out') * (size(enc(a::l)) + size(enc init) + size(enc env))) at 2. *)
-          (*2: {clear IHl. rewrite list_size_cons. cbn; nia. }*)
-
-          (*rewrite list_size_cons at 7. rewrite list_size_cons at 10. solverec. *)
-       (** clear IHl. intros. apply H5 with (l' := a::l'). firstorder. *)
-    (*- subst f; split; smpl_inO. apply inOPoly_comp; smpl_inO. *)
-(*  Qed. *)
-  Admitted. 
+    induction l. 
+    - cbn -[c__fold_right]. lia. 
+    - cbn -[c__fold_right]. rewrite IHl. clear IHl.
+      2: { intros. specialize (H3 (a::l') l''). apply H3. rewrite H2. eauto. } 
+      rewrite G1. 
+      unfold monotonic in *. erewrite G2. 
+      2: { rewrite H3. 2: assert (a::l = [a] ++l) as -> by eauto; easy.
+           erewrite F2. 2: (replace_le (size (enc l)) with (size (enc (a::l))) by (rewrite list_size_cons; lia)); reflexivity. 
+           replace_le (size (enc a)) with (size (enc (a::l))) by (rewrite list_size_cons; lia). 
+           instantiate (1 := (f__size (size (enc (a :: l)) + size (enc env)) + (| l |) * f__size (size (enc (a :: l)) + size (enc env)) + size (enc init) + size (enc (a :: l)) + size (enc env))). 
+           nia. 
+        } 
+      setoid_rewrite G2 at 2. 
+      2: { 
+        instantiate (1 := (f__size (size (enc (a :: l)) + size (enc env)) + (| l |) * f__size (size (enc (a :: l)) + size (enc env)) + size (enc init) + size (enc (a :: l)) + size (enc env))).
+        rewrite F2. 2: (replace_le (size(enc l)) with (size (enc (a::l))) by (rewrite list_size_cons; lia)); reflexivity. 
+        replace_le (size (enc l)) with (size (enc (a::l))) by (rewrite list_size_cons; lia). lia.
+      } 
+      nia.
+  Qed. 
 End fixXY.
-
-
-(*We now fix variants where the environment is not important*)
-Require Import Undecidability.L.Datatypes.LUnit.
-Section noEnv.
-  Context {X : Type}.
-  Context {H : registered X}.
-  (*Lemma list_in_decb_time_bound (eqbT : X -> X -> nat) :*)
-    (*(exists (f : nat -> nat), (forall (a b : X), eqbT a b <= f(size(enc a) + size(enc b))) /\ inOPoly f /\ monotonic f)*)
-      (*-> exists (f : nat -> nat), (forall (l : list X) (e : X), list_in_decb_time eqbT l e <= f(size(enc l) + size(enc e))) /\ inOPoly f /\ monotonic f. *)
-  (*Proof.*)
-    (*intros (f' & H1 & H2 & H3). *)
-    (*assert (exists (f' : nat -> nat), (forall (a b : X) (y : unit), eqbT a b <= f'(size(enc a) + size(enc b) + size(enc y))) /\ inOPoly f' /\ monotonic f').*)
-    (*{ exists f'. split.*)
-      (*+ intros a b y. rewrite H1. unfold monotonic in H3. apply H3. lia.*)
-      (*+ tauto. *)
-    (*}*)
-    (*specialize (list_in_decb_time_bound_env H0) as (f & F1 & F2 & F3). *)
-    (*exists (fun n => f (n + 2)). [> Compute (size (enc tt)) evaluates to 2<]*)
-    (*split. *)
-    (*+ intros. rewrite <- size_unit_enc. apply F1. *)
-    (*+ split; smpl_inO. apply inOPoly_comp; smpl_inO. *)
-  (*Qed. *)
-
-  (*Lemma dupfreeb_time_bound (eqbT : X -> X -> nat):*)
-    (*(exists (f : nat -> nat), (forall (a b : X), eqbT a b <= f (size(enc a) + size(enc b))) /\ inOPoly f /\ monotonic f)*)
-    (*-> exists (f : nat -> nat), (forall (l : list X), dupfreeb_time eqbT l <= f (size(enc l))) /\ inOPoly f /\ monotonic f. *)
-  (*Proof.*)
-    (*intros (f' & H1 & H2 & H3).*)
-    (*assert (exists (f' : nat -> nat),(forall (a b : X) (y : unit), eqbT a b <= f' (size(enc a) + size(enc b) + size(enc y))) /\ inOPoly f' /\ monotonic f').*)
-    (*{ exists f'; split.*)
-      (*- intros; rewrite H1. unfold monotonic in H3. apply H3. lia.*)
-      (*- tauto.*)
-    (*}*)
-    (*specialize (dupfreeb_time_bound_env H0) as (f & F1 & F2 & F3). *)
-    (*exists (fun n => f (n + 2)). [> Compute (size (enc tt)) evaluates to 2<]*)
-    (*split. *)
-    (*+ intros. now rewrite <- size_unit_enc.*)
-    (*+ split; smpl_inO. apply inOPoly_comp; smpl_inO. *)
-  (*Qed. *)
-
-  (*Lemma forallb_time_bound (predT : X -> nat) :*)
-    (*(exists (f : nat -> nat), (forall (a : X),  predT a  <= f (size(enc a))) /\ inOPoly f /\ monotonic f)*)
-    (*-> exists (f : nat -> nat), (forall (l : list X), forallb_time predT l <= f(size (enc l))) /\ inOPoly f /\ monotonic f.*)
-  (*Proof. *)
-    (*intros (f' & H1 & H2 & H3).*)
-    (*assert (exists (f' : nat -> nat),(forall (a : X) (y : unit), (fun (_ : unit) a=> predT a) y a <= f' (size(enc a) + size(enc y))) /\ inOPoly f' /\ monotonic f').*)
-    (*{ exists f'; split.*)
-      (*- intros; rewrite H1. unfold monotonic in H3. apply H3. lia.*)
-      (*- tauto.*)
-    (*}*)
-    (*specialize (forallb_time_bound_env H0) as (f & F1 & F2 & F3). *)
-    (*exists (fun n => f (n + 2)). [> Compute (size (enc tt)) evaluates to 2<]*)
-    (*split. *)
-    (*+ intros. now rewrite <- size_unit_enc.*)
-    (*+ split; smpl_inO. apply inOPoly_comp; smpl_inO. *)
-  (*Qed. *)
-
-  (*Variable (Y : Type).*)
-  (*Context {H0 : registered Y}. *)
-  (*Lemma fold_right_time_bound (step : Y -> X -> X) (stepT : Y -> X -> nat) :*)
-    (*(exists (f : nat -> nat), (forall (acc : X) (ele : Y), stepT ele acc <= f(size(enc acc) + size(enc ele))) /\ inOPoly f /\ monotonic f)*)
-    (*-> (exists (f_size : nat -> nat), (forall (acc : X) (ele : Y), size(enc (step ele acc)) <= size(enc acc) + f_size(size(enc ele))) /\ inOPoly f_size /\ monotonic f_size)*)
-    (*-> exists (f : nat -> nat), (forall (l : list Y) (acc : X), fold_right_time step stepT l acc <= f(size(enc l) + size(enc acc))) /\ inOPoly f /\ monotonic f.*)
-  (*Proof.*)
-    (*intros (f' & H1 & H2 & H3).*)
-    (*intros (f_size & F1 & F2 & F3). *)
-    (*assert (exists (f : nat -> nat), (forall (acc : X) (ele : Y) (env : unit), stepT ele acc <= f(size(enc acc) + size(enc ele) + size(enc env))) /\ inOPoly f /\ monotonic f). *)
-    (*{*)
-      (*exists f'; split. *)
-      (*- intros; rewrite H1. unfold monotonic in H3. apply H3. lia. *)
-      (*- split; smpl_inO. *)
-    (*}*)
-    (*assert (exists (f_size: nat->nat), (forall (acc : X) (ele : Y) (env : unit), size(enc (step ele acc)) <= size(enc acc) + f_size((size(enc ele) + size(enc env)))) /\ inOPoly f_size /\ monotonic f_size).*)
-    (*{*)
-      (*exists f_size. split; [ | easy]. intros. rewrite F1. unfold monotonic in F3. rewrite F3 with (x' := size(enc ele) + size(enc env)); nia. *)
-    (*}*)
-    (*specialize (fold_right_time_bound_env H4 H5) as (f & G1 & G2 & G3).*)
-    (*exists (fun n => f (n + 2)). *)
-    (*split.*)
-    (*- intros. rewrite G1 with (env := tt). now rewrite <- size_unit_enc. *)
-    (*- split; smpl_inO. apply inOPoly_comp; smpl_inO. *)
-  (*Qed. *)
-End noEnv.
 
